Added new rule semax_cast_load to primitive separation logic for C, for load commands that do a cast.

progs/float.c
@@ -1,11 +1,13 @@
 
 
-struct foo {int x; float y;};
+struct foo {int x; float y; double z;};
 
-struct foo s = {5, 3.41};
+struct foo s = {5, 3.41, 0.0};
 
 int main() {
- float y1 = s.y;
+ double y1 = s.y;
  int x1 = s.x;
+ int y2 = s.y;
+ y1 = s.z;
  return 0;
 }
