progs/float.v
@@ -2,31 +2,34 @@ Require Import Clightdefs.
 
 Local Open Scope Z_scope.
 
-Definition _x1 : ident := 15%positive.
+Definition _y1 : ident := 15%positive.
 Definition ___builtin_fabs : ident := 7%positive.
 Definition ___builtin_negl : ident := 3%positive.
 Definition ___builtin_write16_reversed : ident := 1%positive.
-Definition _y1 : ident := 14%positive.
+Definition _s : ident := 14%positive.
 Definition ___builtin_annot_intval : ident := 9%positive.
 Definition ___builtin_addl : ident := 4%positive.
+Definition _y2 : ident := 17%positive.
 Definition ___builtin_memcpy_aligned : ident := 8%positive.
-Definition _main : ident := 16%positive.
-Definition _s : ident := 13%positive.
+Definition _main : ident := 18%positive.
+Definition _x1 : ident := 16%positive.
+Definition _struct_foo : ident := 13%positive.
 Definition ___builtin_mull : ident := 6%positive.
-Definition _struct_foo : ident := 12%positive.
-Definition _x : ident := 11%positive.
+Definition _x : ident := 12%positive.
+Definition _y : ident := 11%positive.
 Definition ___builtin_subl : ident := 5%positive.
 Definition ___builtin_write32_reversed : ident := 2%positive.
-Definition _y : ident := 10%positive.
+Definition _z : ident := 10%positive.
 
 Definition t_struct_foo :=
-   (Tstruct _struct_foo (Fcons _x tint (Fcons _y tfloat Fnil)) noattr).
+   (Tstruct _struct_foo
+     (Fcons _x tint (Fcons _y tfloat (Fcons _z tdouble Fnil))) noattr).
 
 Definition v_s := {|
   gvar_info := t_struct_foo;
   gvar_init := (Init_int32 (Int.repr 5) ::
                 Init_float32 (Float.double_of_bits (Int64.repr 4614861056357957632)) ::
-                nil);
+                Init_float64 (Float.double_of_bits (Int64.repr 0)) :: nil);
   gvar_readonly := false;
   gvar_volatile := false
 |}.
@@ -35,13 +38,17 @@ Definition f_main := {|
   fn_return := tint;
   fn_params := nil;
   fn_vars := nil;
-  fn_temps := ((_y1, tfloat) :: (_x1, tint) :: nil);
+  fn_temps := ((_y1, tdouble) :: (_x1, tint) :: (_y2, tint) :: nil);
   fn_body :=
 (Ssequence
-  (Sset _y1 (Ecast (Efield (Evar _s t_struct_foo) _y tfloat) tfloat))
+  (Sset _y1 (Efield (Evar _s t_struct_foo) _y tfloat))
   (Ssequence
     (Sset _x1 (Efield (Evar _s t_struct_foo) _x tint))
-    (Sreturn (Some (Econst_int (Int.repr 0) tint)))))
+    (Ssequence
+      (Sset _y2 (Ecast (Efield (Evar _s t_struct_foo) _y tfloat) tint))
+      (Ssequence
+        (Sset _y1 (Efield (Evar _s t_struct_foo) _z tdouble))
+        (Sreturn (Some (Econst_int (Int.repr 0) tint)))))))
 |}.
 
 Definition prog : Clight.program := {|
